denotational/System.v
@@ -3,36 +3,17 @@ From Coq Require Import
      Fin
      Relations.
 
-From Equations Require Import Equations.
-
-From ITree Require Import
-     Indexed.Sum
-     Subevent
-     CategoryOps.
+From ExtLib Require Import
+     RelDec
+     String.
 
 From CTree Require Import
-     CTree
-     Equ
-     SBisim
-     Core.Utils
-     Interp.State.
+     Core.Utils.
+  
+From Coq Require Import
+     Fin.
 
-From ExtLib Require Import
-     Maps
-     FMapAList
-     RelDec
-     String
-     Monad.
-
-From Coinduction Require Import
-     coinduction rel tactics.
-
-From DSL Require Import Vectors.
-
-Import MonadNotation EquNotations SBisimNotations.
-Local Open Scope monad_scope.
-Local Open Scope string_scope.
-
+From Equations Require Import Equations.
 Set Implicit Arguments.
 
 (** Some general Sets needed for Systems work *)
@@ -70,6 +51,8 @@ Module DistrSystem <: Systems.
     reldec_uid F1 F1 := true;
     reldec_uid (FS i) (FS j) := reldec_uid i j;
     reldec_uid _ _ := false.
+
+  Transparent reldec_uid.
   
   (** Decidable UIDs *)
   Global Instance eqdec_uid: forall t, RelDec (@eq (uid t)) := {
@@ -87,140 +70,3 @@ Module DistrSystem <: Systems.
     fun T => _.
  
 End DistrSystem.
-
-Module Messaging(S: Systems).
-  Import S.
-
-  Section ParametricN.
-    Variable (n: nat).
-
-    (** Messages exchagend *)
-    Record Msg := {
-        principal: uid n;
-        payload: bytestring
-      }.
-
-    (** Decidable messages *)
-    Global Instance eqdec_msg: RelDec (@eq Msg) := {
-      rel_dec m1 m2 := match m1, m2 with
-                         {| principal := u1; payload := p1 |},
-                         {| principal := u2; payload := p2 |} =>
-                           andb (rel_dec u1 u2) (rel_dec p1 p2)
-                       end      
-    }.
-
-    (** A queue of messages *)
-    Definition queue := list Msg.
-
-    (** A task is either running or returned *)
-    Inductive Task (E: Type -> Type) :=
-    | Running (c: ctree E void)(q: queue)
-    | Blocked (k: option Msg -> ctree E void).
-    (** this is a "soft" blocked -- the scheduler can pass it "None"
-        which corresponds to a timeout, and it will unblock *)
-
-    (** Network effects *)
-    Inductive Net: Type -> Type :=
-    | Recv: Net (option Msg)
-    | Send : Msg -> Net unit
-    | Broadcast: bytestring -> Net unit.    
-  End ParametricN.
-
-  Arguments Running {n} {E}.
-  Arguments Blocked {n} {E}.
-  Arguments Send {n}.
-  Arguments Recv {n}.
-  Arguments Broadcast {n}.
-  
-  Definition recv {E n} `{Net n -< E}: ctree E (option (Msg n)) := trigger Recv.
-  Definition send {E n} `{Net n -< E}: Msg n -> ctree E unit :=
-    fun m => trigger (Send m).
-  Definition broadcast {E n} `{Net n -< E}: bytestring -> ctree E unit :=
-    fun bs => trigger (Broadcast bs).
-
-End Messaging.
-
-Module PKI(S: Systems).
-  Import S.
-  Context {n: nat}.
-
-  Definition Enc (p: uid n) := bytestring.
-  Definition Sig (p: uid n) := bytestring.
-  Definition Pub (p: uid n) := bytestring.
-  Definition Priv (p: uid n) := bytestring.
-  
-  Inductive PKI: Type -> Type :=
-  | EncPub(p: uid n)(k: Pub p)(plain: bytestring): PKI (Enc p)
-  | DecPriv(p: uid n)(k: Priv p)(cipher: Enc p): PKI bytestring
-  | SignPriv(p: uid n)(k: Priv p)(plain: bytestring): PKI (Sig p)
-  | CheckPub(p: uid n)(k: Pub p)(signed: Sig p): PKI bool.
-
-  Definition encrypt {E} `{PKI -< E} := embed EncPub.
-  Definition decrypt {E} `{PKI -< E} := embed DecPriv.
-  Definition sign {E} `{PKI -< E} := embed SignPriv.
-  Definition check {E} `{PKI -< E} := embed CheckPub.
-End PKI.
-
-Module Spawn(S: Systems).
-  Import S.
-
-  Inductive spawnE E : Type -> Type :=
-  | Spawn : forall T (c: channel T) (t: ctree (spawnE E +' E) T), spawnE E (channel T)
-  | Make: forall (T: Type), spawnE E (channel T)
-  | Block: forall T (c: channel T), spawnE E T.
-
-  Definition spawn {F E T} `{(spawnE F) -< E} (c: channel T)(t:ctree (spawnE F +' F) T) :=
-    trigger (@Spawn F T c t).
-  
-  Definition make {F E T} `{(spawnE F) -< E} :=
-    trigger (@Make F T).
-  
-  Definition block {F E} `{(spawnE F) -< E} {t} (c: channel t) :=
-    trigger (@Block F t c).
-  
-End Spawn.  
-
-Module Storage(S: Systems).
-  Import S Monads.
-
-  Definition Map_heap := Map_alist eqdec_var bytestring.
-  Global Existing Instance Map_heap.
-  
-  Notation heap := (alist var bytestring).
-  Notation Storage := (stateE heap).
-
-  Definition load {E} `{stateE heap -< E}(v: var): ctree E (option bytestring) :=
-    get >>= fun s => ret (lookup v s).
-
-  Definition store {E} `{Storage -< E}(v: var)(b: bytestring): ctree E unit :=
-    get >>= fun s => put (add v b s).
-
-  (** Evaluates, takes a single heap for all agents *)
-  Definition run_storage{E R m}(a: vec m (ctree (Storage +' E) R)):
-    stateT heap (fun T => vec m (ctree E T)) R :=
-    fun st => Vector.map (fun it => run_state it st) a.
-  
-End Storage.
-
-Module Log(S: Systems).
-  Import S Monads.
-
-  Inductive logE (S: Type): Type -> Type :=
-  | Log: S -> logE S unit.
-
-  Definition h_state_to_log {E S}: stateE S ~> stateT S (ctree (logE S +' E)) :=
-    fun _ e s =>
-      match e with
-      | Get _ => Ret (s, s)
-      | Put s' => Vis (inl1 (Log s')) (fun _: unit => Ret (s', tt))
-      end.
-
-  Definition pure_state_to_log {S E} : E ~> stateT S (ctree (logE S +' E))
-    := fun _ e s => Vis (inr1 e) (fun x => Ret (s, x)).
-
-  Definition run_state {E S}
-    : ctree (stateE S +' E) ~> stateT S (ctree (logE S +' E))
-    := interp_state (case_ h_state_to_log pure_state_to_log).
-
-End Log.
-
