denotational/Spawn.v
@@ -1,0 +1,32 @@
+From ITree Require Import
+     Indexed.Sum
+     Subevent
+     CategoryOps.
+
+From CTree Require Import
+     CTree.
+
+From DSL Require Import System.
+
+Set Implicit Arguments.
+
+Module Spawn(S: Systems).
+  Import S.
+
+  Inductive spawnE E : Type -> Type :=
+  | Spawn : forall T (c: channel T) (t: ctree (spawnE E +' E) T), spawnE E (channel T)
+  | Make: forall (T: Type), spawnE E (channel T)
+  | Block: forall T (c: channel T), spawnE E T.
+
+  Definition spawn {F E T} `{(spawnE F) -< E} (c: channel T)(t:ctree (spawnE F +' F) T) :=
+    trigger (@Spawn F T c t).
+  
+  Definition make {F E T} `{(spawnE F) -< E} :=
+    trigger (@Make F T).
+  
+  Definition block {F E} `{(spawnE F) -< E} {t} (c: channel t) :=
+    trigger (@Block F t c).
+  
+End Spawn.  
+
+
