denotational/Storage.v
@@ -1,0 +1,92 @@
+From Coq Require Import
+     String
+     Fin
+     Relations.
+
+From ITree Require Import
+     Indexed.Sum
+     Subevent
+     CategoryOps.
+
+From CTree Require Import
+     CTree
+     Interp.State.
+
+From ExtLib Require Import
+     Maps
+     FMapAList
+     RelDec
+     String
+     Monad.
+
+From DSL Require Import Vectors Lists System.
+
+Import MonadNotation.
+Local Open Scope monad_scope.
+Local Open Scope string_scope.
+Local Open Scope fin_vector_scope.
+
+Set Implicit Arguments.
+
+(** This is not your standard state monad,
+    as daemons do not return, ever. We instead interpret
+    state *changes* as Visible log events. So this is a transformer
+    from stateE S -> logE S *) 
+Module Storage(S: Systems).
+  Import S Monads.
+
+  Notation heap := (alist var bytestring).
+  Notation Storage := (stateE heap).
+  
+  Global Instance Map_heap: Map var bytestring heap := Map_alist eqdec_var bytestring.
+
+  (** Equality of heaps is extensional (functional extensionality)
+      for all keys in either one, values must match *)
+  Global Instance eqdec_heap: RelDec (@eq heap) := {
+      rel_dec a b :=
+      let fix rec (a' b': heap) := 
+        match a' with
+        | ((k, v) :: ts)%list => match alist_find _ k b with
+                        | Some v' => andb (rel_dec v v') (rec ts b')
+                        | None => false
+                        end
+        | nil%list=> true
+        end in
+      andb (rec a b) (rec b a)
+    }.
+  
+  Definition load {E} `{stateE heap -< E}(v: var): ctree E (option bytestring) :=
+    get >>= fun s => ret (lookup v s).
+
+  Definition store {E} `{Storage -< E}(v: var)(b: bytestring): ctree E unit :=
+    get >>= fun s => put (add v b s).
+  
+  Section ParametricS.
+    Context {S: Type} {dec_S: RelDec (@eq S)}.
+
+    Inductive logE (S: Type): Type -> Type :=
+    | Log: S -> logE S unit.
+
+    Definition h_state_to_log {E}: stateE S ~> stateT S (ctree (logE S +' E)) :=
+      fun _ e s =>
+        match e with
+        | Get _ => Ret (s, s)
+        | Put s' => if rel_dec s s' then
+                     Ret (s, tt) else
+                     Vis (inl1 (Log s')) (fun _: unit => Ret (s', tt))
+        end.
+
+    Definition pure_state_to_log {E} : E ~> stateT S (ctree (logE S +' E))
+      := fun _ e s => Vis (inr1 e) (fun x => Ret (s, x)).
+
+    Definition run_state {E}: ctree (stateE S +' E) ~> stateT S (ctree (logE S +' E))
+      := interp_state (case_ h_state_to_log pure_state_to_log).
+
+    Definition run_states {n E R}(v: vec n (ctree (stateE S +' E) R)):
+      stateT S (fun T => vec n (ctree (logE S +' E) T)) R :=
+      fun st => Vector.map (fun a => run_state a st) v.
+    
+  End ParametricS.
+
+End Storage.
+
